@prefix adms: <http://www.w3.org/ns/adms#> .
@prefix clvapit: <https://w3id.org/italia/onto/CLV/> .
@prefix dcat: <http://www.w3.org/ns/dcat#> .
@prefix dcatapit: <http://dati.gov.it/onto/dcatapit#> .
@prefix dct: <http://purl.org/dc/terms/> .
@prefix foaf: <http://xmlns.com/foaf/0.1/> .
@prefix inailvoc: <https://w3id.org/italia/work-accident/controlled-vocabulary/proc6_pdda1/> .
@prefix ndc: <https://w3id.org/italia/onto/NDC/> .
@prefix owl: <http://www.w3.org/2002/07/owl#> .
@prefix rdfs: <http://www.w3.org/2000/01/rdf-schema#> .
@prefix skos: <http://www.w3.org/2004/02/skos/core#> .
@prefix stpratica: <https://w3id.org/italia/work-accident/controlled-vocabulary/proc6_pdda1/stato_pratica_pdda1/concetto/> .
@prefix vcard: <http://www.w3.org/2006/vcard/ns#> .
@prefix xkos: <http://rdf-vocabulary.ddialliance.org/xkos#> .
@prefix xsd: <http://www.w3.org/2001/XMLSchema#> .

### Annotations

<https://w3id.org/italia/data/standard/SKOS> a dcatapit:Standard,
        dct:Standard ;
    dct:description "The Simple Knowledge Organization System (SKOS) is a common data model for sharing and linking knowledge organization systems via the Web" ;
    dct:identifier "SKOS" ;
    dct:title "Simple Knowledge Organization System - SKOS" .

<https://w3id.org/italia/work-accident/data/organization/inail> a dcatapit:Agent,
        foaf:Agent ;
    dct:identifier "inail" ;
    foaf:name "Istituto Nazionale per l'Assicurazione contro gli Infortuni sul Lavoro"@it,
        "National Institute for Insurance against Accidents at Work"@en .

<https://w3id.org/italia/work-accident/data/organization/ufficioV> a dcatapit:Organization,
        vcard:Kind,
        vcard:Organization ;
    vcard:fn "INAIL Ufficio V - D.C.O.D" ;
    vcard:hasEmail <mailto:dcod@inail.it> .

<https://w3id.org/italia/work-accident/data/proc6_pdda1/distribution/STP_CSV> a dcat:Distribution,
        dcatapit:Distribution ;
    dcat:accessURL <https://github.com/InailUfficio5/inail-ndc/tree/main/assets/controlled-vocabularies/stato_pratica_pdda1/v1.0> ;
    dcat:downloadURL <https://raw.githubusercontent.com/InailUfficio5/inail-ndc/main/assets/controlled-vocabularies/stato_pratica_pdda1/v1.0/stato_pratica_pdda1.csv> ;
    dct:description "Questa è la distribuzione CSV del vocabolario controllato sulla classificazione delle tipologie di stato della pratica della richiesta relativa al documento PDDA1 adottata dall'INAIL"@it,
        "This is the distribution in CSV of the classification of the status types of the PD DA1 document-related request procedure adopted by INAIL controlled vocabulary"@en ;
    dct:format <http://publications.europa.eu/resource/authority/file-type/CSV> ;
    dct:license <https://w3id.org/italia/controlled-vocabulary/licences/A21_CCBY40> ;
    dct:title "CSV distribution of the classification of the status types of the PD DA1 document-related request procedure adopted by INAIL controlled vocabulary"@en,
        "Distribuzione CSV del vocabolario controllato sulla classificazione delle tipologie di stato della pratica della richiesta relativa al documento PDDA1 adottata dall'INAIL"@it .

<https://w3id.org/italia/work-accident/data/proc6_pdda1/distribution/STP_JSON> a dcat:Distribution,
        dcatapit:Distribution ;
    dcat:accessURL <https://github.com/InailUfficio5/inail-ndc/tree/main/assets/controlled-vocabularies/stato_pratica_pdda1/v1.0> ;
    dcat:downloadURL <https://raw.githubusercontent.com/InailUfficio5/inail-ndc/main/assets/controlled-vocabularies/stato_pratica_pdda1/v1.0/stato_pratica_pdda1.json> ;
    dct:description "Questa è la distribuzione JSON del vocabolario controllato sulla classificazione delle tipologie di stato della pratica della richiesta relativa al documento PDDA1 adottata dall'INAIL"@it,
        "This is the distribution in JSON of the classification of the status types of the PD DA1 document-related request procedure adopted by INAIL controlled vocabulary"@en ;
    dct:format <http://publications.europa.eu/resource/authority/file-type/JSON> ;
    dct:license <https://w3id.org/italia/controlled-vocabulary/licences/A21_CCBY40> ;
    dct:title "Distribuzione JSON del vocabolario controllato sulla classificazione delle tipologie di stato della pratica della richiesta relativa al documento PDDA1 adottata dall'INAIL"@it,
        "JSON distribution of the classification of the status types of the PD DA1 document-related request procedure adopted by INAIL controlled vocabulary"@en .

<https://w3id.org/italia/work-accident/data/proc6_pdda1/distribution/STP_RDF_TURTLE> a dcat:Distribution,
        dcatapit:Distribution ;
    dcat:accessURL <https://github.com/InailUfficio5/inail-ndc/tree/main/assets/controlled-vocabularies/stato_pratica_pdda1/v1.0> ;
    dcat:downloadURL <https://raw.githubusercontent.com/InailUfficio5/inail-ndc/main/assets/controlled-vocabularies/stato_pratica_pdda1/v1.0/stato_pratica_pdda1.ttl> ;
    dct:description "Questa è la distribuzione RDF/Turtle del vocabolario controllato sulla classificazione delle tipologie di stato della pratica della richiesta relativa al documento PDDA1 adottata dall'INAIL"@it,
        "This is the distribution in RDF/turtle of the classification of the status types of the PD DA1 document-related request procedure adopted by INAIL controlled vocabulary"@en ;
    dct:format <http://publications.europa.eu/resource/authority/file-type/RDF_TURTLE> ;
    dct:license <https://w3id.org/italia/controlled-vocabulary/licences/A21_CCBY40> ;
    dct:title "Distribuzione RDF/Turtle del vocabolario controllato sulla classificazione delle tipologie di stato della pratica della richiesta relativa al documento PDDA1 adottata dall'INAIL"@it,
        "RDF/Turtle distribution of the classification of the status types of the PD DA1 document-related request procedure adopted by INAIL controlled vocabulary"@en .

inailvoc:stato_pratica_pdda1 a adms:Asset,
        dcatapit:Dataset,
        skos:ConceptScheme ;
    rdfs:label "This is the controlled vocabulary of the status types of the PD DA1 document-related request procedure adopted by INAIL classification"@en,
        "Vocabolario Controllato sulla classificazione delle tipologie di stato della pratica della richiesta relativa al documento PDDA1 adottata dall'INAIL"@it ;
    skos:prefLabel "Vocabolario Controllato sulla classificazione delle tipologie di stato della pratica della richiesta relativa al documento PDDA1 adottata dall'INAIL"@it ;
    rdfs:comment "Status types of the PD DA1 document-related request procedure: Closed, Data not Available, To Work, Under Investigation, Sent, Sent with Errors, Suspended, Substituted"@en,
        "Tipologie di stato della pratica della richiesta relativa al documento PDDA1: Chiusa, Dato non Disponibile, Da Lavorare, In Istruttoria, Inviata, Inviata con Errori, Sospesa, Sostituita"@it ;
    owl:versionInfo "0.1" ;
    rdfs:isDefinedBy inailvoc:stato_pratica_pdda1 ;
    adms:representationTechnique <http://purl.org/adms/representationtechnique/SKOS> ;
    dcat:contactPoint <https://w3id.org/italia/work-accident/data/organization/ufficioV> ;
    dcat:distribution <https://w3id.org/italia/work-accident/data/proc6_pdda1/distribution/STP_CSV>,
        <https://w3id.org/italia/work-accident/data/proc6_pdda1/distribution/STP_JSON>,
        <https://w3id.org/italia/work-accident/data/proc6_pdda1/distribution/STP_RDF_TURTLE> ;
    dcat:keyword "bureaucracy"@en,
        "burocrazia"@it,
        "document"@en,
        "documento"@it,
        "inail"@it,
        "pd da1"@it,
        "pratica"@it,
        "procedure"@en ;
    dcat:theme <http://publications.europa.eu/resource/authority/data-theme/ECON>,
        <http://publications.europa.eu/resource/authority/data-theme/SOCI> ;
    dct:accrualPeriodicity <http://publications.europa.eu/resource/authority/frequency/IRREG> ;
    dct:conformsTo <https://w3id.org/italia/data/standard/SKOS> ;
    dct:creator <https://w3id.org/italia/work-accident/data/organization/inail> ;
    dct:description "Status types of the PD DA1 document-related request procedure: Closed, Data not Available, To Work, Under Investigation, Sent, Sent with Errors, Suspended, Substituted"@en,
        "Tipologie di stato della pratica della richiesta relativa al documento PDDA1: Chiusa, Dato non Disponibile, Da Lavorare, In Istruttoria, Inviata, Inviata con Errori, Sospesa, Sostituita"@it ;
    dct:identifier "https://w3id.org/italia/work-accident/controlled-vocabulary/proc6_pdda1/stato_pratica_pdda1" ;
    dct:issued "2023-08-28"^^xsd:date ;
    dct:language <http://publications.europa.eu/resource/authority/language/ITA> ;
    dct:modified "2023-08-31"^^xsd:date ;
    dct:publisher <https://w3id.org/italia/work-accident/data/organization/inail> ;
    dct:relation <https://w3id.org/italia/work-accident/controlled-vocabulary/adm_serv/definizione_amministrativa> ;
    dct:rightsHolder <https://w3id.org/italia/work-accident/data/organization/inail> ;
    dct:subject <http://eurovoc.europa.eu/100234>,
        <http://eurovoc.europa.eu/100236> ;
    dct:title "Classification of the status types of the PD DA1 document-related request procedure adopted by INAIL controlled vocabulary"@en,
        "Vocabolario Controllato sulla classificazione delle tipologie di stato della pratica della richiesta relativa al documento PDDA1 adottata dall'INAIL"@it ;
    dct:type <http://purl.org/adms/assettype/CodeList> ;
    ndc:keyConcept "stato_pratica_pdda1" ;
    skos:hasTopConcept stpratica:1,
        stpratica:2,
        stpratica:3,
        stpratica:4,
        stpratica:5,
        stpratica:6,
        stpratica:7,
        stpratica:8 ;
    xkos:numberOfLevels "1" .

stpratica:1 a skos:Concept ;
    rdfs:label "Sostituita"@it ;
    skos:prefLabel "Sostituita"@it ;
    clvapit:hasRankOrder "1" ;
    dct:identifier "1" ;
    skos:inScheme inailvoc:stato_pratica_pdda1 ;
    skos:notation "1" ;
    xkos:depth "1" .

stpratica:2 a skos:Concept ;
    rdfs:label "Sospesa"@it ;
    skos:prefLabel "Sospesa"@it ;
    clvapit:hasRankOrder "1" ;
    dct:identifier "2" ;
    skos:inScheme inailvoc:stato_pratica_pdda1 ;
    skos:notation "2" ;
    xkos:depth "1" .

stpratica:3 a skos:Concept ;
    rdfs:label "Chiusa"@it ;
    skos:prefLabel "Chiusa"@it ;
    clvapit:hasRankOrder "1" ;
    dct:identifier "3" ;
    skos:inScheme inailvoc:stato_pratica_pdda1 ;
    skos:notation "3" ;
    xkos:depth "1" .

stpratica:4 a skos:Concept ;
    rdfs:label "Inviata"@it ;
    skos:prefLabel "Inviata"@it ;
    clvapit:hasRankOrder "1" ;
    dct:identifier "4" ;
    skos:inScheme inailvoc:stato_pratica_pdda1 ;
    skos:notation "4" ;
    xkos:depth "1" .

stpratica:5 a skos:Concept ;
    rdfs:label "In Istruttoria"@it ;
    skos:prefLabel "In Istruttoria"@it ;
    clvapit:hasRankOrder "1" ;
    dct:identifier "5" ;
    skos:inScheme inailvoc:stato_pratica_pdda1 ;
    skos:notation "5" ;
    xkos:depth "1" .

stpratica:6 a skos:Concept ;
    rdfs:label "Inviata con Errori"@it ;
    skos:prefLabel "Inviata con Errori"@it ;
    clvapit:hasRankOrder "1" ;
    dct:identifier "6" ;
    skos:inScheme inailvoc:stato_pratica_pdda1 ;
    skos:notation "6" ;
    xkos:depth "1" .

stpratica:7 a skos:Concept ;
    rdfs:label "Da Lavorare"@it ;
    skos:prefLabel "Da Lavorare"@it ;
    clvapit:hasRankOrder "1" ;
    dct:identifier "7" ;
    skos:inScheme inailvoc:stato_pratica_pdda1 ;
    skos:notation "7" ;
    xkos:depth "1" .

stpratica:8 a skos:Concept ;
    rdfs:label "Dato non Disponibile"@it ;
    skos:prefLabel "Dato non Disponibile"@it ;
    clvapit:hasRankOrder "1" ;
    dct:identifier "8" ;
    skos:inScheme inailvoc:stato_pratica_pdda1 ;
    skos:notation "8" ;
    xkos:depth "1" .

### Serialized using the ttlser deterministic serializer v1.2.0
